Update.

src/metalogic/paper.lean
@@ -9,6 +9,25 @@ import data.finset
 set_option pp.parens true
 
 
+def fin_zip
+	{α β : Type}
+	[decidable_eq α]
+	(σ : α → β) : Π (n : ℕ), (fin n → α) → (fin n → β) → (α → β)
+| 0 _ _ := σ
+| (n + 1) f g :=
+	function.update
+		(fin_zip n (fun (i : fin n), (f i)) (fun (i : fin n), (g i)))
+		(f n) (g n)
+
+def fin_map
+	{α β : Type}
+	(m : α → β)
+	(n : ℕ)
+	(f : fin n → α) :
+	(fin n → β) :=
+	fun (i : fin n), m (f i)
+
+
 abbreviation var_name := ℕ
 abbreviation func_name := string
 abbreviation pred_name := string
@@ -30,9 +49,18 @@ inductive formula : Type
 open formula
 
 
+-- sub_var_term_single x t t0 = t0 [x / t]
 def sub_var_term_single (x : var_name) (t : term) : term → term
 | (var y) := if y = x then t else var y
 | (func n f ts) := func n f (fun (i : fin n), sub_var_term_single (ts i))
+
+
+-- (((t0 [x1 / t1]) [x2 / t2]) ... [xn / tn])
+def sub_var_term_single_repeat (t0 : term) : Π n : ℕ, (fin n → var_name) → (fin n → term) → term
+| 0 _ _ := t0
+| (n + 1) xs ts :=
+	sub_var_term_single (xs n) (ts n)
+		(sub_var_term_single_repeat n (fun (i : fin n), (xs i)) (fun (i : fin n), (ts i)))
 
 
 structure interpretation (ω : Type) : Type :=
@@ -40,6 +68,7 @@ structure interpretation (ω : Type) : Type :=
 (var : var_name → ω)
 (func (n : ℕ) : func_name → ((fin n → ω) → ω))
 (pred (n : ℕ) : pred_name → ((fin n → ω) → Prop))
+
 
 def interpretation.var_update
 	{ω : Type}
@@ -54,6 +83,22 @@ def interpretation.var_update
 		pred := I.pred
 	}
 
+
+def interpretation.var_update_repeat
+	{ω : Type}
+	(I : interpretation ω)
+	(n : ℕ)
+	(xs : fin n → var_name)
+	(ds : fin n → ω) :
+	interpretation ω :=
+	{
+		nonempty := I.nonempty,
+		var := fin_zip I.var n xs ds,
+		func := I.func,
+		pred := I.pred
+	}
+
+
 def interpretation.term {ω : Type} (I : interpretation ω) : term → ω
 | (var x) := I.var x
 | (func n f t) := I.func n f (fun (i : fin n), interpretation.term (t i))
@@ -62,7 +107,6 @@ def interpretation.term {ω : Type} (I : interpretation ω) : term → ω
 def term.all_var_set : term → finset var_name
 | (var x) := {x}
 | (func n f t) := finset.univ.bUnion (fun (i : fin n), (t i).all_var_set)
-
 
 
 lemma lem_1_a
@@ -101,4 +145,19 @@ begin
 		congr, funext,
 		exact ih i,
 	},
+end
+
+lemma lem_1_b
+	(n : ℕ)
+	(zs : fin n → var_name)
+	(nodup : function.injective zs)
+	(ts : fin n → term)
+	(h1 : ∀ (i j : fin n), (zs i) ∉ (ts j).all_var_set)
+	(ω : Type)
+	(I : interpretation ω)
+	(t0 : term) :
+	(I.var_update_repeat n zs (fin_map I.term n ts)).term t0 =
+		I.term (sub_var_term_single_repeat t0 n zs ts) :=
+begin
+	admit
 end
